proofs/toEC/toEC_jazz.v
@@ -1,20 +1,22 @@
-Require Import compiler_util expr.
+Require Import compiler_util expr arch_decl arch_extra.
 Require Import normalize_cond.
 Require Import refresh_for.
 Require Import for_to_while.
 Require Import flatten_while.
+Require Import remove_baseop_casts.
 
 Section TOEC.
 
 Context
-  {asm_op : Type}
-  {asmop : asmOp asm_op}
+  {reg regx xreg rflag cond asm_op extra_op : Type}
+  {asm_e : asm_extra reg regx xreg rflag cond asm_op extra_op}
   (fresh_var_ident : v_kind -> instr_info -> string -> atype -> Ident.ident)
 .
 
 Definition toEC_prog (normal : bool) (p : _uprog) : cexec _uprog :=
   Let p1 := refresh_for_prog fresh_var_ident false (normalize_cond_prog p) in
   Let p2 := if normal then for_to_while_prog fresh_var_ident p1 else ok p1 in
-  ok (flatten_while_prog p2).
+  let p3 := flatten_while_prog p2 in
+  remove_baseop_casts_prog fresh_var_ident p3.
 
 End TOEC.
