compiler/examples/extraction-unit-tests/proofs.ec
@@ -46,45 +46,6 @@ hoare t_empty_range_counter_correct :
   For_to_while.M.t_empty_range_counter : true ==> res = W32.of_int 42.
 proof. by proc; rcondf ^while; auto. qed.
 
-hoare t_while_pre_correct :
-  Flatten_while.M.t_while_pre : true ==> res = W32.of_int 6.
-proof.
-  proc; wp.
-  while (c = i + 1 /\ 0 <= i <= 5).
-  - by auto => /#.
-  by auto => /#.
-qed.
-
-hoare t_nested_while_pre_correct :
-  Flatten_while.M.t_nested_while_pre : true ==> res = W32.of_int 9.
-proof.
-  proc; wp.
-  while (0 <= i <= 3 /\ j = 0 /\ c = 3 * i).
-  - wp.
-    while (0 <= j <= 2 /\ c = 3 * i + 1 + j).
-    - by auto => /#.
-    by auto => /#.
-  by auto => /#.
-qed.
-
-hoare t_do_while_correct :
-  Flatten_while.M.t_do_while : true ==> res = W32.of_int 4.
-proof.
-  proc; wp.
-  while (c = i /\ 0 <= i <= 4).
-  - by auto => /#.
-  by auto => /#.
-qed.
-
-hoare t_plain_while_correct :
-  Flatten_while.M.t_plain_while : true ==> res = W32.of_int 5.
-proof.
-  proc; wp.
-  while (c = i /\ 0 <= i <= 5).
-  - by auto => /#.
-  by auto => /#.
-qed.
-
 lemma sdiv_correct : hoare [ Sdiv.M.main: true ==> res = (W64.of_int (-1), W64.of_int (-1)) ].
 proof.
   proc; auto => _ _.
